revived all proofs with late approximation (in tome domain) most error terms got simpler. need to reflect that in the paper improved the format of the table in the figure

icreate.v
@@ -1392,8 +1392,8 @@ Qed.
 Local Opaque approximate CRmult.
 Lemma ThetaAtEV1 :
      (|{theta ic} mt1 - optimalTurnAngle|) ≤ 
-          Q2R (rotspeed * (2 * (sendTimeAcc + delivDelayVar) 
-                  + reacTime + R2QPrec) 
+          Q2R (rotspeed * (R2QPrec+ 2 * (sendTimeAcc + delivDelayVar) 
+                  + reacTime) 
               + (motorTurnOmegaPrec ω) * (mt1 - mt0))%Q.
 Proof.
   pose proof correctVel0to1 as Hc.
@@ -1477,28 +1477,23 @@ Qed.
 
 Require Export Coq.QArith.Qabs.
 
+Definition timeErr : Q := 
+  (R2QPrec + 2 * (sendTimeAcc + delivDelayVar))%Q.
+
 Lemma MotorEv01Gap3 :
-   AbsIR ((Q2R (QT2Q mt1 - QT2Q mt0)) 
-      - ((CRasIR (CRabs (polarTheta targetPos))) * (Qinv rotspeed)))
-  [<=] Q2R ((anglePrec* (Qinv rotspeed)) + 2 * (sendTimeAcc + delivDelayVar)).
+   AbsIR ((Q2R (QT2Q mt1 - QT2Q mt0)) - 'rotDuration)
+  [<=] Q2R timeErr.
 Proof.
-  pose proof  MotorEv01Gap  as Hg.
-  fold mt0 mt1 in Hg.
-  simpl in Hg.
+  pose proof  MotorEv01Gap  as Hg. unfold timeErr.
   apply (inj_Q_leEq IR) in Hg.
   rewrite <- AbsIR_Qabs in Hg.
   rewrite cgminus_Qminus, inj_Q_minus in Hg.
-  pose proof (approximateAbsSmallIR 
-      (CRabs (polarTheta targetPos)) anglePrec) as Hball.
-  rewrite approximate_CRabs in Hball.
+  pose proof (approximateAbsSmallIR  rotDuration R2QPrec) as Hball.
+  apply AbsIR_imp_AbsSmall in Hg.
   apply AbsSmall_minus in Hball.
-  apply mult_resp_AbsSmallR with (y:= Q2R (Qinv rotspeed)) in Hball;
-    [| apply QposDivLe0IR].
-  rewrite  IRDistMinus in Hball.
-  autorewrite with QSimpl in Hball.
+  unfold Q2R in Hball.
 Local Opaque CRabs.
   simpl in Hball.
-  apply AbsIR_imp_AbsSmall in Hg.
   pose proof (AbsSmall_plus _ _ _ _ _  Hg Hball) as Hadd.
   clear Hball Hg.
   unfold Q2R, cg_minus in Hadd.
@@ -1512,13 +1507,11 @@ Local Opaque CRabs.
   unfold Mult_instance_IR.
   eapply AbsSmall_morph_wd;
     [| | apply Hadd].
-- apply inj_Q_wd. simpl. ring.
+- apply inj_Q_wd. simpl. unfold timeErr. ring.
 - unfold Q2R, Qminus, cg_minus. reflexivity.
 Qed.
 
-Definition Ev01TimeGapUB : IR :=
-  ((CRasIR (CRabs (polarTheta targetPos)) + anglePrec) * (Qinv rotspeed))
-  + E2EDelVar.
+Definition Ev01TimeGapUB : IR := 'rotDuration + Q2R timeErr.
 
 Lemma MotorEv01Gap4 :
    Q2R (QT2Q mt1 - QT2Q mt0) ≤ Ev01TimeGapUB.
@@ -1531,34 +1524,20 @@ Proof.
   apply proj2 in Hp.
   apply shift_leEq_plus in Hp.
   unfold Ev01TimeGapUB.
-  eapply leEq_transitive;[apply Hp|].
-  clear Hp.
-  unfold E2EDelVar.
-  unfoldMC.
-  autounfold with IRMC.
-  unfold Mult_instance_IR.
-  rewrite ring_distl_unfolded.
-  simpl. idtac. destruct sendTimeAcc, delivDelayVar.
-  simpl. apply eqImpliesLeEq.
-  simpl.  
-  autorewrite with QSimpl. simpl.
-  Local Transparent Q2R.
-  unfold Q2R. 
-  rewrite inj_Q_plus.
-  ring.
+  rewrite plus_comm.
+  exact Hp.
 Qed.
 
 Hint Resolve qtimePosIR : ROQCOQ.
 Lemma ThetaAtEV1_2 :
      (|{theta ic} mt1 - optimalTurnAngle|) ≤ 
-          Q2R (rotspeed * (2 * (sendTimeAcc + delivDelayVar) + reacTime) +
-               anglePrec)%Q + (Q2R (motorTurnOmegaPrec ω) * Ev01TimeGapUB).
+          Q2R (rotspeed * (timeErr + reacTime))
+            + (Q2R (motorTurnOmegaPrec ω) * Ev01TimeGapUB).
 Proof.
   intros. pose proof ThetaAtEV1 as Hom.
   Local Opaque Qabs.Qabs Q2R.
   simpl in Hom.
   Local Transparent Q2R.
-  fold mt0 mt1 in Hom.
   eapply leEq_transitive;[apply Hom|].
   unfold Q2R. unfoldMC.
   rewrite inj_Q_plus. 
@@ -1577,29 +1556,53 @@ Qed.
 Lemma ThetaAtEV1_3 :
   let omPrec : Q :=  (eeew 0%Q ω) in 
  |{theta ic} mt1 - optimalTurnAngle| ≤ 
-   Q2R(rotspeed * (E2EDelVar + reacTime) 
-    + anglePrec + omPrec * E2EDelVar)
-    + Q2R (omPrec / rotspeed)%Q * ('(CRabs (polarTheta targetPos)) + Q2R anglePrec).
+   Q2R(rotspeed * (timeErr + reacTime) +
+    omPrec * timeErr)
+    + Q2R (omPrec / rotspeed)%Q * ('(CRabs (polarTheta targetPos))).
 Proof.
   Local Opaque Q2R.
   simpl.
   pose proof ThetaAtEV1_2 as Hev.
   simpl in Hev.
   eapply leEq_transitive;[apply Hev|].
+  Local Transparent Q2R.
+  unfold Q2R.
+  rewrite inj_Q_plus.
+  autounfold with IRMC.
+  rewrite <- plus_assoc_unfolded.
+  apply plus_resp_leEq_lft.
   apply eq_imp_leEq.
   unfold Ev01TimeGapUB.
   fold E2EDelVar.
   unfold eeew, motorTurnOmegaPrec.
   remember (θ (motorPrec {| rad := 0%Q; θ := ω |}) ) as ew.
   unfold cast, Cart_CR_IR.
-  remember (CRasIR (CRabs (polarTheta targetPos))) as crabs.
+  unfold rotDuration, CanonicalNotations.norm,
+  NormSpace_instance_0.
   unfoldMC.
   autounfold with IRMC.
+  Local Opaque Q2R.
+  simpl.
+  rewrite CR_mult_asIR.
+  remember (CRasIR (CRabs (polarTheta targetPos))) as crabs.
   autorewrite with QSimpl.
+  unfold Qdiv.
+
+(* delete *)
+Lemma CRasIRInj : ∀ q,
+  CRasIR (inject_Q_CR q) = inj_Q IR q.
+Proof.
+  intros.
+  apply (injective IRasCR).
+  rewrite CRasIRasCR_id.
+  autorewrite with IRtoCR.
+  reflexivity.
+Qed.
+Hint Rewrite CRasIRInj : CRtoIR.
+  autorewrite with CRtoIR.
+  autorewrite with InjQDown.
   Local Transparent Q2R.
   unfold Q2R.
-  unfold Qdiv.
-  autorewrite with InjQDown.
   ring.
 Qed.
 
@@ -1684,9 +1687,9 @@ Qed.
 Local Opaque Q2R.
 
 Definition θErrTurn : IR :=
-Q2R (rotspeed * (E2EDelVar + 2 * reacTime) 
-  + anglePrec + (eeew 0%Q ω) * (E2EDelVar + reacTime))%Q
-    + Q2R ((eeew 0%Q ω) / rotspeed)%Q * ('(CRabs (polarTheta targetPos)) + Q2R anglePrec).
+Q2R(rotspeed * (timeErr + 2* reacTime) +
+    (eeew 0%Q ω) * (timeErr + reacTime))
+    + Q2R ((eeew 0%Q ω) / rotspeed)%Q * ('(|polarTheta targetPos|)).
 
 Lemma ThetaAtEV2 :
  (|{theta ic} mt2 - optimalTurnAngle|) ≤ θErrTurn.
@@ -1739,6 +1742,8 @@ Proof.
   unfold motorTurnOmegaPrec, eeew.
   remember (θ (motorPrec {| rad := 0%Q; θ := ω |})) as ew.
   simpl.
+  unfold rotDuration, CanonicalNotations.norm,
+  NormSpace_instance_0.
   ring.
 Qed.
 
@@ -1894,51 +1899,42 @@ Proof.
   assumption.
 Qed.
 
+Definition transDuration : CR :=  ((| targetPos |) * '(/speed)%Q).
+
+
 Lemma MotorEv23Gap :
-  let t0 : QTime := MotorEventsNthTime 2 (decAuto (2<4)%nat I) in
-  let t1 : QTime := MotorEventsNthTime 3 (decAuto (3<4)%nat I) in
-  let tgap :Q := (approximate (|targetPos|) distPrec * (Qinv speed)) in
-   |QT2Q t1 - QT2Q t0 -  tgap| 
-  ≤ 2 * (sendTimeAcc + delivDelayVar)%Q.
+   (|QT2Q mt3 - QT2Q mt2 -  approximate transDuration R2QPrec|)
+   ≤ 2 * (sendTimeAcc + delivDelayVar)%Q.
 Proof.
-  intros ? ? ?.
   apply MotorEvGap.
 Qed.
 
-Definition Ev23TimeGapUB : IR :=
-  ((CRasIR ((|targetPos|)) + distPrec) * (Qinv speed))
-  + E2EDelVar.
+Definition Ev23TimeGapUB : IR := 'transDuration + Q2R timeErr.
 
-Definition θErrTrans : IR :=
-(QT2R rotErrTrans) * Ev23TimeGapUB.
 
-Lemma MotorEv23Gap2_2 :
-  let t0 : QTime := MotorEventsNthTime 2 (decAuto (2<4)%nat I) in
-  let t1 : QTime := MotorEventsNthTime 3 (decAuto (3<4)%nat I) in
-   AbsIR ((Q2R (QT2Q t1 - QT2Q t0)) 
-      - ((CRasIR (|targetPos|)) * (Qinv speed)))
-  [<=] Q2R ((distPrec* (Qinv speed)) + 2 * (sendTimeAcc + delivDelayVar)).
+Definition θErrTrans : IR := (QT2R rotErrTrans) * Ev23TimeGapUB.
+
+
+Lemma MotorEv23Gap3 :
+   AbsIR ((Q2R (QT2Q mt3 - QT2Q mt2)) - 'transDuration) 
+  [<=] timeErr.
 Proof.
-  intros ? ? .
-  pose proof  MotorEv23Gap  as Hg.
-  simpl in Hg.
-  fold t0 t1 in Hg.
+  pose proof  MotorEv23Gap  as Hg. unfold timeErr.
   apply (inj_Q_leEq IR) in Hg.
   rewrite <- AbsIR_Qabs in Hg.
   rewrite cgminus_Qminus, inj_Q_minus in Hg.
-  pose proof (approximateAbsSmallIR (|targetPos |) distPrec) as Hball.
-  apply AbsSmall_minus in Hball.
-  apply mult_resp_AbsSmallR with (y:= Q2R (Qinv speed)) in Hball;
-    [| apply QposDivLe0IR].
-  rewrite  IRDistMinus in Hball.
-  autorewrite with QSimpl in Hball.
-  simpl in Hball.
+  pose proof (approximateAbsSmallIR  transDuration R2QPrec) as Hball.
   apply AbsIR_imp_AbsSmall in Hg.
+  apply AbsSmall_minus in Hball.
+  unfold Q2R in Hball.
+Local Opaque CRabs.
+  simpl in Hball.
   pose proof (AbsSmall_plus _ _ _ _ _  Hg Hball) as Hadd.
   clear Hball Hg.
   unfold Q2R, cg_minus in Hadd.
   simpl in Hadd. revert Hadd.
   unfoldMC. intro Hadd.
+  unfold CanonicalNotations.norm, NormSpace_instance_Q in Hadd.
   ring_simplify in Hadd.
   autounfold with IRMC.
   apply AbsSmall_imp_AbsIR.
@@ -1946,18 +1942,14 @@ Proof.
   unfold Mult_instance_IR.
   eapply AbsSmall_morph_wd;
     [| | apply Hadd].
-- apply inj_Q_wd. simpl. ring.
+- apply inj_Q_wd. simpl. unfold timeErr. ring.
 - unfold Q2R, Qminus, cg_minus. reflexivity.
 Qed.
 
-Lemma MotorEv23Gap2_3 :
-  let t2 : QTime := MotorEventsNthTime 2 (decAuto (2<4)%nat I) in
-  let t3 : QTime := MotorEventsNthTime 3 (decAuto (3<4)%nat I) in
-   Q2R (QT2Q t3 - QT2Q t2) ≤ Ev23TimeGapUB.
+Lemma MotorEv23Gap4 :
+   Q2R (QT2Q mt3 - QT2Q mt2) ≤ Ev23TimeGapUB.
 Proof.
-  intros ? ?.
-  pose proof MotorEv23Gap2_2 as Hp.
-  fold t2 t3 in Hp.
+  pose proof MotorEv23Gap3 as Hp.
   Local Opaque Q2R.
   simpl in Hp.
   apply AbsIR_imp_AbsSmall in Hp.
@@ -1965,35 +1957,16 @@ Proof.
   apply proj2 in Hp.
   apply shift_leEq_plus in Hp.
   unfold Ev23TimeGapUB.
-  eapply leEq_transitive;[apply Hp|].
-  clear Hp.
-  unfold E2EDelVar.
-  unfoldMC.
-  autounfold with IRMC.
-  unfold Mult_instance_IR.
-  rewrite ring_distl_unfolded.
-  simpl. idtac. destruct sendTimeAcc, delivDelayVar.
-  simpl. apply eqImpliesLeEq.
-  simpl.  
-  autorewrite with QSimpl. simpl.
-  Local Transparent Q2R.
-  unfold Q2R. 
-  rewrite inj_Q_plus.
-  ring.
+  rewrite plus_comm.
+  exact Hp.
 Qed.
 
-Definition Ev23TimeGapLB : IR :=
-  ((CRasIR ((|targetPos|)) - QposAsQ distPrec) * (Qinv speed))
-  - E2EDelVar.
 
-Lemma MotorEv23GapLB :
-  let t2 : QTime := MotorEventsNthTime 2 (decAuto (2<4)%nat I) in
-  let t3 : QTime := MotorEventsNthTime 3 (decAuto (3<4)%nat I) in
-   Ev23TimeGapLB  ≤  Q2R (t3 - t2).
+Definition Ev23TimeGapLB : IR := 'transDuration - Q2R timeErr.
+
+Lemma MotorEv23GapLB : Ev23TimeGapLB  ≤  Q2R (mt3 - mt2).
 Proof.
-  intros ? ?.
-  pose proof MotorEv23Gap2_2 as Hp.
-  fold t2 t3 in Hp.
+  pose proof MotorEv23Gap3 as Hp.
   Local Opaque Q2R.
   simpl in Hp.
   apply AbsIR_imp_AbsSmall in Hp.
@@ -2002,25 +1975,9 @@ Proof.
   apply shift_plus_leEq in Hp.
   unfold Ev23TimeGapLB.
   eapply leEq_transitive;[|apply Hp].
-  clear Hp.
-  unfold E2EDelVar.
   unfoldMC.
   autounfold with IRMC.
-  unfold Mult_instance_IR.
-  rewrite ring_distl_unfolded.
-  simpl.  destruct sendTimeAcc, delivDelayVar.
-  simpl. apply eqImpliesLeEq.
-  simpl.  
-  autorewrite with QSimpl. simpl.
-  Local Transparent Q2R.
-  unfold Q2R. 
-  rewrite inj_Q_inv.
-  rewrite inj_Q_inv.
-  pose proof QDivQopp as Hq.
-  unfold Qdiv in Hq.
-  rewrite <- Hq.
-  rewrite inj_Q_inv.
-  rewrite inj_Q_plus.
+  apply eqImpliesLeEq. unfold cast, Cart_CR_IR.
   ring.
 Qed.
 
@@ -2037,7 +1994,7 @@ Proof.
   rewrite inj_Q_mult in Hb.
   eapply leEq_transitive;[apply Hb|].
   eapply mult_resp_leEq_lft;[| eauto with ROSCOQ; fail].
-  apply MotorEv23Gap2_3.
+  apply MotorEv23Gap4.
 Qed.
 
 Lemma ThetaEv2To3_3 :
@@ -2609,7 +2566,7 @@ Proof.
   cbv zeta in Hyd.
   eapply leEq_transitive;[apply Hyd|].
   clear Hyd.
-  apply mult_resp_leEq_rht;[apply MotorEv23Gap2_3; fail|].
+  apply mult_resp_leEq_rht;[apply MotorEv23Gap4; fail|].
   eapply leEq_transitive;[apply AbsIR_nonneg| apply YDerivEv2To3].
   instantiate (1:=MotorEventsNthTime 2 (decAuto (2 < 4)%nat I)).
   unfold le, Le_instance_QTime.
@@ -2643,9 +2600,9 @@ Qed.
 Lemma YChangeEv2To3_3 :
   AbsIR ({Y rotOrigininPos} mt3 [-] {Y rotOrigininPos} mt2) 
       ≤ (Sin (θErrTrans + θErrTurn) * 
-        ((CRasIR (|targetPos |) + distPrec) 
+        (('(|targetPos |)) 
           + Ev23TimeGapUB * QT2R transErrTrans
-          + Q2R speed * E2EDelVar)).
+          + Q2R speed * timeErr)).
 Proof.
   intros.
   pose proof (YChangeEv2To3_2) as Hyd.
@@ -2653,14 +2610,17 @@ Proof.
   eapply leEq_transitive;[apply Hyd|].
   clear Hyd.
   apply eqImpliesLeEq.
-  unfold Ev23TimeGapUB.
+  unfold Ev23TimeGapUB, transDuration.
   unfoldMC. autounfold with IRMC.
   rewrite mult_commut_unfolded, <- mult_assoc_unfolded.
   apply mult_wdr.
   unfold QT2R, Q2R.
   rewrite inj_Q_plus.
   ring_simplify.
-  rewrite qpCancel.
+  unfold cast, Cart_CR_IR.
+  rewrite CR_mult_asIR.
+  rewrite CRasIRInj.
+  rewrite mult_assoc_unfolded.
   rewrite qpCancel.
   ring_simplify.
   autorewrite with InjQDown.
@@ -2680,7 +2640,7 @@ Qed.
 
 
 Definition ErrY': IR :=  '(eeev 0 ω) * (QT2R reacTime + Ev01TimeGapUB)
-+ (Sin (θErrTrans + θErrTurn)) * (CRasIR (|targetPos |) + distPrec + Ev23TimeGapUB * '(eeev speed 0) + (Q2R speed) * E2EDelVar).
++ (Sin (θErrTrans + θErrTurn)) * ('(|targetPos |) + Ev23TimeGapUB * '(eeev speed 0) + (Q2R speed) * timeErr).
 
 Lemma Ev3Y' : AbsIR ({Y rotOrigininPos} mt3)  ≤ ErrY'.
 Proof.
@@ -2778,7 +2738,7 @@ Proof.
   eapply leEq_transitive;[apply Hyd|].
   fold t2 t3. clear Hyd.
   unfold Q2R. rewrite inj_Q_mult.
-  apply mult_resp_leEq_rht;[apply MotorEv23Gap2_3; fail|].
+  apply mult_resp_leEq_rht;[apply MotorEv23Gap4; fail|].
   eauto 2 with CoRN ROSCOQ.
 Qed.
 
@@ -2932,7 +2892,7 @@ Lemma Liveness :
       ts < t → (|(posAtTime t) - targetPosR|) ≤ cast Q IR acceptableDist.
 Abort.
 
-sEnd iCREATECPS.
+End iCREATECPS.
 End RobotProgam.
 
 
